adapted to 2020-RC1

thys/examples/code/euclid.ll
@@ -12,47 +12,39 @@ define i64 @euclid(i64 %a, i64 %b) {
   start:
     %x = insertvalue { i64, i64 } zeroinitializer, i64 %a, 0
     %xa = insertvalue { i64, i64 } %x, i64 %b, 1
-    %xb = call { i64, i64 } @LLVM_Examples_euclid_f_04204230 ({ i64, i64 } %xa)
+    br label %while_start
+
+  while_start:
+    %xb = phi { i64, i64 } [ %x6, %ctd_if ], [ %xa, %start ]
     %a1 = extractvalue { i64, i64 } %xb, 0
+    %x1 = extractvalue { i64, i64 } %xb, 1
+    %x2 = icmp ne i64 %a1, %x1
+    br i1 %x2, label %while_body, label %while_end
+
+  while_body:
+    %a2 = extractvalue { i64, i64 } %xb, 0
     %b1 = extractvalue { i64, i64 } %xb, 1
-    ret i64 %a1
-}
-
-define { i64, i64 } @LLVM_Examples_euclid_f_04204230({ i64, i64 } %s) {
-
-  start:
-    %a = extractvalue { i64, i64 } %s, 0
-    %x = extractvalue { i64, i64 } %s, 1
-    %ctd = icmp ne i64 %a, %x
-    br i1 %ctd, label %then, label %else
+    %tmpa = icmp ule i64 %a2, %b1
+    br i1 %tmpa, label %then, label %else
 
   then:
-    %a1 = extractvalue { i64, i64 } %s, 0
-    %b = extractvalue { i64, i64 } %s, 1
-    %tmpa = icmp ule i64 %a1, %b
-    br i1 %tmpa, label %thena, label %elsea
-
-  thena:
-    %xaa = insertvalue { i64, i64 } zeroinitializer, i64 %a1, 0
-    %x1 = sub i64 %b, %a1
-    %x2 = insertvalue { i64, i64 } %xaa, i64 %x1, 1
-    br label %ctd_ifa
-
-  elsea:
-    %xc = sub i64 %a1, %b
-    %xaa1 = insertvalue { i64, i64 } zeroinitializer, i64 %xc, 0
-    %x3 = insertvalue { i64, i64 } %xaa1, i64 %b, 1
-    br label %ctd_ifa
-
-  ctd_ifa:
-    %x4 = phi { i64, i64 } [ %x3, %elsea ], [ %x2, %thena ]
-    %x5 = call { i64, i64 } @LLVM_Examples_euclid_f_04204230 ({ i64, i64 } %x4)
+    %xaa = insertvalue { i64, i64 } zeroinitializer, i64 %a2, 0
+    %x3 = sub i64 %b1, %a2
+    %x4 = insertvalue { i64, i64 } %xaa, i64 %x3, 1
     br label %ctd_if
 
   else:
+    %xc = sub i64 %a2, %b1
+    %xaa1 = insertvalue { i64, i64 } zeroinitializer, i64 %xc, 0
+    %x5 = insertvalue { i64, i64 } %xaa1, i64 %b1, 1
     br label %ctd_if
 
   ctd_if:
-    %x6 = phi { i64, i64 } [ %s, %else ], [ %x5, %ctd_ifa ]
-    ret { i64, i64 } %x6
+    %x6 = phi { i64, i64 } [ %x5, %else ], [ %x4, %then ]
+    br label %while_start
+
+  while_end:
+    %a3 = extractvalue { i64, i64 } %xb, 0
+    %b2 = extractvalue { i64, i64 } %xb, 1
+    ret i64 %a3
 }
